Begin conversion
Signed-off-by: zeramorphic <zeramorphic@proton.me>

ConNF/Counting/Spec.lean
@@ -18,7 +18,7 @@ variable [Params.{u}] [Level] [FOAAssumptions] {β : Λ}
 
 inductive SpecCondition (β : Λ)
   | atom (A : ExtendedIndex β) (s : Set κ) (t : Set κ)
-  | flexible (A : ExtendedIndex β) (s : Set κ)
+  | flexible (A : ExtendedIndex β) (s : Set κ) (t : κ → Set κ)
   | inflexibleCoe (A : ExtendedIndex β) (h : InflexibleCoePath A)
       (χ : CodingFunction h.δ) (hχ : χ.Strong) (t : κ → Set κ)
   | inflexibleBot (A : ExtendedIndex β) (h : InflexibleBotPath A) (s : Set κ) (t : κ → Set κ)
@@ -53,7 +53,10 @@ structure Specifies (σ : Spec β) (S : Support β) (hS : S.Strong) : Prop where
       Flexible A N.1 →
       S.f i hi = ⟨A, inr N⟩ →
       σ.f i (hi.trans_eq max_eq_max) = SpecCondition.flexible A
-        {j | ∃ hj, ∃ (N' : NearLitter), S.f j hj = ⟨A, inr N⟩ ∧ N'.1 = N'.1}
+        {j | ∃ hj, ∃ (N' : NearLitter), S.f j hj = ⟨A, inr N'⟩ ∧ N'.1 = N.1}
+        (fun j => {k | ∃ hj hk, ∃ (a : Atom) (N' : NearLitter),
+          N'.1 = N.1 ∧ a ∈ (N : Set Atom) ∆ N' ∧
+          S.f j hj = ⟨A, inr N'⟩ ∧ S.f k hk = ⟨A, inl a⟩})
   inflexibleCoe_spec (i : κ) (hi : i < S.max) (A : ExtendedIndex β) (N : NearLitter)
       (h : InflexibleCoe A N.1) (hSi : S.f i hi = ⟨A, inr N⟩) :
       σ.f i (hi.trans_eq max_eq_max) = SpecCondition.inflexibleCoe A h.path
@@ -88,8 +91,8 @@ theorem Specifies.of_eq_atom {σ : Spec β} {S : Support β} {hS : S.Strong} (h 
   · cases hi'.symm.trans (h.inflexibleCoe_spec i hiS B N hN hc.symm)
 
 theorem Specifies.of_eq_flexible {σ : Spec β} {S : Support β} {hS : S.Strong} (h : σ.Specifies S hS)
-    {i : κ} {hi : i < σ.max} {A : ExtendedIndex β} {s : Set κ}
-    (hi' : σ.f i hi = SpecCondition.flexible A s) :
+    {i : κ} {hi : i < σ.max} {A : ExtendedIndex β} {s : Set κ} {t : κ → Set κ}
+    (hi' : σ.f i hi = SpecCondition.flexible A s t) :
     ∃ N, Flexible A N.1 ∧ S.f i (hi.trans_eq h.max_eq_max.symm) = ⟨A, inr N⟩ := by
   have hiS := hi.trans_eq h.max_eq_max.symm
   set c := S.f i hiS with hc
